src/BinEncoders/Env/Examples/UDP_Packet.v
@@ -23,7 +23,8 @@ Require Import
         Fiat.BinEncoders.Env.Lib2.NatOpt
         Fiat.BinEncoders.Env.Lib2.Vector
         Fiat.BinEncoders.Env.Lib2.EnumOpt
-        Fiat.BinEncoders.Env.Lib2.SumTypeOpt.
+        Fiat.BinEncoders.Env.Lib2.SumTypeOpt
+        Fiat.BinEncoders.Env.Lib2.IPChecksum.
 
 Require Import Bedrock.Word.
 
@@ -38,24 +39,322 @@ Definition UDP_Packet :=
           "DestPort" :: word 16, (* Don't fragment flag *)
           "Payload" :: list char >.
 
-Variable IPChecksum : ByteString -> ByteString.
-
 Definition transformer : Transformer ByteString := ByteStringTransformer.
 
-Definition UDPChecksum (* Dummy Checksum for now*)
+Definition UDP_Checksum_Valid
            (srcAddr : word 32)
            (destAddr : word 32)
-           (udpLength : nat)
+           (udpLength : word 16)
+           (n : nat)
            (b : ByteString)
-  := ByteString_id.
+  := IPChecksum_Valid (96 + n)
+                (transform (transform (encode_word' 32 srcAddr)
+                (transform (encode_word' 32 destAddr)
+                (transform (encode_word' 8 (wzero 8))
+                (transform (encode_word' 8 (natToWord 8 17))
+                           (encode_word' 16 udpLength)))))
+                b).
 
 Definition encode_UDP_Packet_Spec
            (srcAddr : word 32)
            (destAddr : word 32)
+           (udpLength : word 16)
            (* These values are provided by the IP header for checksum calculation.*)
            (udp : UDP_Packet) :=
-          encode_word_Spec (udp!"SourcePort")
+          (encode_word_Spec (udp!"SourcePort")
     ThenC encode_word_Spec (udp!"DestPort")
-    ThenC encode_nat_Spec 16 (64 + |udp!"Payload"|) (* payload length is an argument *)
-    ThenChecksum (UDPChecksum srcAddr destAddr (64 + |udp!"Payload"|))
-    ThenCarryOn encode_list_Spec encode_word_Spec udp!"Payload".
+    ThenC encode_nat_Spec 16 (8 + |udp!"Payload"|) DoneC)
+    ThenChecksum (UDP_Checksum_Valid srcAddr destAddr udpLength) OfSize 16
+    ThenCarryOn (encode_list_Spec encode_word_Spec udp!"Payload"
+             ThenC (if (Peano_dec.eq_nat_dec (NPeano.modulo (length udp!"Payload") 2) 0) then encode_word_Spec WO else encode_word_Spec (wzero 8))
+                                  DoneC).
+
+Definition UDP_Packet_OK (udp : UDP_Packet) :=
+  lt (|udp!"Payload"|) (pow2 16 - 8).
+
+Definition UDP_Packet_encoded_measure (udp_b : ByteString)
+  : nat :=
+  match (`(u, b') <- decode_unused_word' 16 udp_b;
+         `(u, b') <- decode_unused_word' 16 b';
+           decode_word' 16 b') with
+  | Some n => 8 * wordToNat (fst n)
+  | None => 0
+  end.
+
+Lemma if_computes_to_len {P}
+  : forall (b : {P} + {~P}) b' encodeT encodeE n n' ctx ctx',
+    (forall b ctx ctx', encodeT ctx ↝ (b, ctx') -> length_ByteString b = n)
+    -> (forall b (ctx ctx' : CacheEncode), encodeE ctx ↝ (b, ctx') -> length_ByteString b = n')
+    -> (if b then encodeT else encodeE) ctx ↝ (b', ctx')
+    -> length_ByteString b' = if b then n else n'.
+Proof.
+  intros; find_if_inside; eauto.
+Qed.
+
+Arguments NPeano.modulo : simpl never.
+
+Lemma mod_16_even_8 :
+  forall n,
+    NPeano.modulo n 2 = 0
+    -> NPeano.modulo (n * 8 + 0) 16 = 0.
+Proof.
+  intros; rewrite <- plus_n_O.
+  rewrite Mult.mult_comm.
+  pose proof (NPeano.Nat.mul_mod_distr_l n 2 8).
+  unfold mult at 2 in H0; simpl in H0.
+  rewrite H0, H; eauto.
+Qed.
+
+Lemma mod_16_odd_8 :
+  forall n,
+    NPeano.modulo n 2 <> 0
+    -> NPeano.modulo (n * 8) 16 = 8.
+Proof.
+  intros; rewrite Mult.mult_comm.
+  pose proof (NPeano.Nat.mul_mod_distr_l n 2 8).
+  unfold mult at 2 in H0; simpl in H0.
+  rewrite H0; eauto.
+  pose proof (NPeano.Nat.mod_upper_bound n 2).
+  omega.
+Qed.
+
+Definition UDP_Packet_decoder'
+  : { decodePlusCacheInv |
+      forall srcAddr destAddr udpLength,
+      exists P_inv,
+        (cache_inv_Property (snd decodePlusCacheInv) P_inv
+         -> encode_decode_correct_f _ transformer UDP_Packet_OK (fun _ _ => True)
+                                    (encode_UDP_Packet_Spec srcAddr destAddr udpLength)
+                                    ((fst decodePlusCacheInv) srcAddr destAddr udpLength)
+                                    (snd decodePlusCacheInv))
+        /\ cache_inv_Property (snd decodePlusCacheInv) P_inv}.
+Proof.
+  eexists (_, _); intros; eexists _; split; simpl.
+  unfold encode_UDP_Packet_Spec; pose_string_ids.
+  intro.
+  let p := (eval unfold Domain in (fun udp : UDP_Packet => (udp!StringId, (udp!StringId0, |udp!StringId1|)))) in
+  let p := eval simpl in p in
+      eapply (@compose_IPChecksum_encode_correct_dep
+                UDP_Packet
+                _
+                _
+                (word 16 * (word 16 * nat))
+                _ _ _ H
+                p
+                UDP_Packet_OK
+                _ _ _
+                (fun data' : word 16 * (word 16 * nat) =>
+                   (encode_word_Spec (fst data')
+              ThenC encode_word_Spec (fst (snd data'))
+              ThenC encode_nat_Spec 16 (8 + (snd (snd data')))
+              DoneC))).
+  simpl transform; rewrite !transform_ByteString_measure, !length_encode_word';
+    reflexivity.
+  reflexivity.
+  repeat calculate_length_ByteString.
+  repeat calculate_length_ByteString.
+  intros. eapply if_computes_to_len; eauto;
+            repeat calculate_length_ByteString.
+  solve_mod_16.
+  intros; cbv beta; find_if_inside.
+  solve_mod_16.
+  simpl; rewrite mod_16_even_8; eauto.
+  solve_mod_16; simpl.
+  intros; rewrite <- NPeano.Nat.add_mod_idemp_l; eauto.
+  simpl; rewrite mod_16_odd_8; eauto.
+  { (* Grossest Proof By Far. *)
+    intros; simpl transform_id; rewrite length_ByteString_ByteString_id.
+    instantiate (1 := UDP_Packet_encoded_measure).
+    unfold UDP_Packet_encoded_measure.
+    rewrite <- !transform_assoc.
+    simpl in H0.
+    eapply computes_to_compose_decode_unused_word in H0;
+      let H' := fresh in
+      destruct H0 as [? [? [? H'] ] ]; rewrite H'.
+    unfold DecodeBindOpt, If_Opt_Then_Else.
+    eapply computes_to_compose_decode_unused_word in H0;
+      let H' := fresh in
+      destruct H0 as [? [? [? H'] ] ]; rewrite H'.
+    unfold DecodeBindOpt, If_Opt_Then_Else.
+    eapply computes_to_compose_decode_word in H0;
+      let H' := fresh in
+      destruct H0 as [? [? [? H'] ] ]; rewrite H'.
+    unfold fst.
+    find_if_inside.
+    rewrite wordToNat_natToWord_idempotent; try reflexivity.
+    rewrite !Plus.plus_assoc.
+    clear.
+    unfold StringId, StringId0, StringId1; clear.
+    repeat match goal with
+      |- context [ @length ?A (GetAttribute ?z ?l)] => remember (@length A (GetAttribute z l))
+    end.
+    assert (n = n0) by (rewrite Heqn, Heqn0; f_equal).
+    rewrite <- H.
+    omega.
+    revert H2; clear; unfold UDP_Packet_OK; intros.
+    revert H2;
+      repeat match goal with
+               |- context [ @length ?A (GetAttribute ?z ?l)] => remember (@length A (GetAttribute z l))
+             end.
+    assert (n = n0) by (rewrite Heqn, Heqn0; f_equal).
+    rewrite <- H.
+    intros; auto with arith.
+    rewrite <- BinNat.N.compare_lt_iff.
+    rewrite Nnat.N2Nat.inj_compare.
+    rewrite Nnat.Nat2N.id.
+    admit.
+    clear; admit.
+  }
+  apply_compose.
+  eapply Word_decode_correct.
+  solve_data_inv.
+  solve_data_inv.
+  apply_compose.
+  eapply Word_decode_correct.
+  solve_data_inv.
+  solve_data_inv.
+  apply_compose.
+  eapply Nat_decode_correct.
+  solve_data_inv.
+  solve_data_inv.
+  unfold encode_decode_correct_f; intuition eauto.
+  simpl in *.
+  instantiate
+    (1 := fun p b env => if Compare_dec.le_lt_dec p (pow2 16) then
+                           _ p b env else None).
+  simpl in *.
+  assert (b0 = proj1 - 8) by
+      (rewrite <- H9; simpl; auto with arith).
+  destruct (Compare_dec.le_lt_dec proj1 (pow2 16)).
+  rewrite H8; clear H8.
+  clear H9.
+  computes_to_inv; injections; subst; simpl.
+  eexists env'; simpl; intuition eauto.
+  rewrite ByteString_transform_id_left.
+  match goal with
+    |- ?f ?a ?b ?c = ?P =>
+    let P' := (eval pattern a, b, c in P) in
+    let f' := match P' with ?f a b c => f end in
+    try unify f f'; try reflexivity
+  end.
+  omega.
+  simpl in H6.
+  find_if_inside; try discriminate.
+  simpl in H6; injections; eauto.
+  simpl.
+  eexists _; eexists tt;
+    intuition eauto; injections; eauto using idx_ibound_eq;
+      try match goal with
+            |-  ?data => destruct data;
+                           simpl in *; eauto
+          end.
+  destruct env; computes_to_econstructor.
+  pose proof transform_id_left as H'; simpl in H'; rewrite H'.
+  find_if_inside; simpl in *; try discriminate;
+    injections.
+  reflexivity.
+  instantiate (1 := fun _ => True); eauto.
+  find_if_inside; try discriminate; injections.
+  clear; admit.
+  find_if_inside; try discriminate; injections; eauto.
+  find_if_inside; try discriminate; injections; eauto.
+  find_if_inside; try discriminate; injections; eauto.
+  clear; admit.
+  unfold UDP_Packet_OK; clear; intros ? H'; repeat split.
+  simpl.
+  clear; admit.
+  instantiate (1 := fun _ _ => True);
+    simpl; intros; exact I.
+  apply_compose.
+  intro H'; eapply FixList_decode_correct.
+  eapply Word_decode_correct.
+  eapply H'.
+  simpl; intros; instantiate (1 := snd (snd proj)).
+  intuition.
+  destruct proj as [? [? ?] ]; simpl; injections; eauto.
+  simpl; intros; eauto using FixedList_predicate_rest_True.
+  intros.
+
+  eapply Word_decode_correct.
+  solve_data_inv.
+  solve_data_inv.
+  apply_compose.
+  intro; eapply FixList_decode_correct.
+  revert H3; eapply Word_decode_correct.
+  simpl in *; split.
+  intuition eauto.
+  eapply (f_equal fst H8).
+  intros; eauto.
+  simpl; intros; eauto using FixedList_predicate_rest_True.
+  simpl; intros;
+    unfold encode_decode_correct_f; intuition eauto.
+  destruct data as [? [? [? [? [? [? [? [? [? [? [ ] ] ] ] ] ] ] ] ] ] ];
+    unfold GetAttribute, GetAttributeRaw in *;
+    simpl in *.
+  pose proof (f_equal fst H14).
+  pose proof (f_equal (fun z => fst (snd z)) H14).
+  pose proof (f_equal (fun z => fst (snd (snd z))) H14).
+  pose proof (f_equal (fun z => fst (snd (snd (snd z)))) H14).
+  pose proof (f_equal (fun z => fst (snd (snd (snd (snd z))))) H14).
+  pose proof (f_equal (fun z => fst (snd (snd (snd (snd (snd z)))))) H14).
+  pose proof (f_equal (fun z => fst (snd (snd (snd (snd (snd (snd z))))))) H14).
+  pose proof (f_equal (fun z => fst (snd (snd (snd (snd (snd (snd z))))))) H14).
+  pose proof (f_equal (fun z => snd (snd (snd (snd (snd (snd (snd z))))))) H14).
+  simpl in *.
+  clear H14.
+  computes_to_inv; injections; subst; simpl.
+  pose proof transform_id_left as H'; simpl in H'; rewrite H'.
+  eexists env'; simpl; intuition eauto.
+  simpl in *.
+  simpl in H8; injections; eauto.
+  simpl in H8; repeat find_if_inside; try discriminate.
+  eexists _; eexists tt.
+  injections; simpl in *; repeat split.
+  destruct env; computes_to_econstructor.
+  pose proof transform_id_left as H'; simpl in H'; rewrite H'.
+  reflexivity.
+  unfold GetAttribute, GetAttributeRaw; simpl.
+  rewrite H5; eauto.
+  intuition.
+  simpl in *.
+  unfold pow2 in H9; simpl in H9; auto with arith.
+  omega.
+  unfold GetAttribute, GetAttributeRaw.
+  simpl.
+  rewrite H5.
+  omega.
+  destruct proj as [? [? [? [? [? [? [? ?] ] ] ] ] ] ].
+  simpl.
+  unfold GetAttribute, GetAttributeRaw; simpl in *.
+  repeat f_equal.
+  eauto.
+  simpl.
+  repeat (instantiate (1 := fun _ => True)).
+  unfold cache_inv_Property; intuition.
+  Grab Existential Variables.
+  decide equality.
+  decide equality.
+  exact (@weq _).
+Defined.
+
+Definition IPv4_decoder_impl :=
+  Eval simpl in (fst (projT1 EthernetHeader_decoder)).
+
+Print IPv4_decoder_impl.
+
+
+Lemma UDP_Packet_Headiner_Len_Bound
+  : forall (a : UDP_Packet) (a_OK : UDP_Packet_OK a),
+    BinNat.N.lt (BinNat.N.of_nat (UDP_Packet_Header_Len a)) (Npow2 4).
+Proof.
+  unfold IPv4_Packet_Header_Len.
+  intros; unfold IPv4_Packet_OK in a_OK.
+  destruct a_OK.
+  rewrite <- BinNat.N.compare_lt_iff.
+  rewrite Nnat.N2Nat.inj_compare.
+  rewrite Nnat.Nat2N.id.
+  rewrite <- Compare_dec.nat_compare_lt.
+  simpl.
+  unfold BinPos.Pos.to_nat; simpl.
+  auto with arith.
+Qed.
