src/BinEncoders/Env/Common/Notations.v
@@ -1,7 +1,7 @@
 Reserved Notation "'Either' t 'Or' e " (at level 100, right associativity).
 Reserved Notation "x 'ThenC' y" (at level 100, right associativity).
 Reserved Notation "x 'DoneC'"   (at level 99, right associativity).
-Reserved Notation "encode1 'ThenChecksum' c 'ThenCarryOn' encode2"
+Reserved Notation "encode1 'ThenChecksum' c 'OfSize' sz 'ThenCarryOn' encode2"
          (encode2 at next level, at level 98, right associativity).
 Reserved Notation "| ls |" (at level 200).
 
